add enfa for cat and star with nfa

theories/enfa.v
@@ -18,41 +18,41 @@ Definition eps_closure {A: Type}
 Section FAs.
   Context {A: finType}.
 
-  Definition nul: t A. refine {|
-    state := state.NZero;
-    start := set0;
-    final := set0;
-    tf ch src dst := false
-  |}.
-  Defined.
+  (* Definition nul: t A. refine {| *)
+  (*   state := state.NZero; *)
+  (*   start := set0; *)
+  (*   final := set0; *)
+  (*   tf ch src dst := false *)
+  (* |}. *)
+  (* Defined. *)
 
-  Definition eps: t A. refine {|
-    state := state.NOne;
-    start := [set tt];
-    final := [set tt];
-    tf ch src dst :=
-      match ch with
-      | None => true
-      | Some c => false
-      end
-  |}.
-  Defined.
+  (* Definition eps: t A. refine {| *)
+  (*   state := state.NOne; *)
+  (*   start := [set tt]; *)
+  (*   final := [set tt]; *)
+  (*   tf ch src dst := *)
+  (*     match ch with *)
+  (*     | None => true *)
+  (*     | Some c => false *)
+  (*     end *)
+  (* |}. *)
+  (* Defined. *)
 
-  Definition char (f: A -> bool): t A. refine {|
-    state := state.NPlus state.NOne state.NOne;
-    start := [set (inl tt)];
-    final := [set (inr tt)];
-    tf ch src dst :=
-      match ch with
-      | None => src == dst
-      | Some c =>
-          match src, dst with
-          | inl _, inr _ => f c
-          | _, _ => false
-          end
-      end
-  |}.
-  Defined.
+  (* Definition char (f: A -> bool): t A. refine {| *)
+  (*   state := state.NPlus state.NOne state.NOne; *)
+  (*   start := [set (inl tt)]; *)
+  (*   final := [set (inr tt)]; *)
+  (*   tf ch src dst := *)
+  (*     match ch with *)
+  (*     | None => src == dst *)
+  (*     | Some c => *)
+  (*         match src, dst with *)
+  (*         | inl _, inr _ => f c *)
+  (*         | _, _ => false *)
+  (*         end *)
+  (*     end *)
+  (* |}. *)
+  (* Defined. *)
 
   Definition cat (n1 n2: t A): t A. refine {|
     state := state.NPlus (state n1) (state n2);
@@ -69,22 +69,22 @@ Section FAs.
   |}.
   Defined.
 
-  Definition alt (n1 n2: t A): t A. refine {|
-    state := state.NPlus (state n1) (state n2);
-    start := (inl @: start n1) :|: (inr @: start n2);
-    final := (inl @: (start n1)) :|: (inr @: (start n2));
-    tf ch src dst := 
-      match ch with
-      | None => src == dst
-      | Some c =>
-          match src, dst with
-          | inl s, inl d => (tf n1) ch s d
-          | inr s, inr d => (tf n2) ch s d
-          | _, _ => false
-          end
-      end
-  |}.
-  Defined.
+  (* Definition alt (n1 n2: t A): t A. refine {| *)
+  (*   state := state.NPlus (state n1) (state n2); *)
+  (*   start := (inl @: start n1) :|: (inr @: start n2); *)
+  (*   final := (inl @: (start n1)) :|: (inr @: (start n2)); *)
+  (*   tf ch src dst := *) 
+  (*     match ch with *)
+  (*     | None => src == dst *)
+  (*     | Some c => *)
+  (*         match src, dst with *)
+  (*         | inl s, inl d => (tf n1) ch s d *)
+  (*         | inr s, inr d => (tf n2) ch s d *)
+  (*         | _, _ => false *)
+  (*         end *)
+  (*     end *)
+  (* |}. *)
+  (* Defined. *)
 
   Definition star (n: t A): t A. refine {|
     state := state.NPlus state.NOne (state n);
